src/Spec/Protocol.v
@@ -29,55 +29,6 @@ Section Protocol.
       op_allow op tid s /\
       lo_step op tid s r s'.
 
-  Inductive exec_any (tid : nat) (s : State) :
-    forall T (p : proc opT T) (r : T) (s' : State), Prop :=
-  | ExecAnyOther :
-    forall T (p : proc opT T) (r : T) (s' : State)
-           T' (op' : opT T') tid' s0 r0,
-    tid <> tid' ->
-    restricted_step op' tid' s r0 s0 ->
-    exec_any tid s0 p r s' ->
-    exec_any tid s p r s'
-  | ExecAnyThisDone :
-    forall T (p : proc opT T) (r : T) (s' : State) evs,
-    exec_tid restricted_step tid s p s' (inl r) evs ->
-    exec_any tid s p r s'
-  | ExecAnyThisMore :
-    forall T (p p' : proc opT T) (s' s0 : State) r evs,
-    exec_tid restricted_step tid s p s0 (inr p') evs ->
-    exec_any tid s0 p' r s' ->
-    exec_any tid s p r s'
-  .
-
-  Definition exec_others (tid : nat) (s s' : State) : Prop :=
-    clos_refl_trans_1n _
-      (fun s0 s1 =>
-        exists tid' `(op' : opT T') r',
-          tid' <> tid /\
-          restricted_step op' tid' s0 r' s1)
-      s s'.
-
-  Lemma exec_any_op : forall `(op : opT T) tid r s s',
-    exec_any tid s (Op op) r s' ->
-      exists s0,
-        exec_others tid s s0 /\
-        restricted_step op tid s0 r s'.
-  Proof.
-    intros.
-    remember (Op op).
-    induction H; subst.
-    - edestruct IHexec_any; eauto; intuition idtac.
-      eexists; split; eauto.
-      econstructor; eauto.
-      do 4 eexists; split.
-      eauto.
-      unfold restricted_step in *; intuition eauto.
-    - exists s; split.
-      eapply rt1n_refl.
-      exec_tid_inv; eauto.
-    - exec_tid_inv.
-  Qed.
-
   Variable loopInv : forall (s : State) (tid : nat), Prop.
 
   Inductive follows_protocol_proc (tid : nat) (s : State) :
@@ -90,7 +41,7 @@ Section Protocol.
     forall T1 T2 (p1 : proc _ T1) (p2 : T1 -> proc _ T2),
     follows_protocol_proc tid s p1 ->
     (forall r s',
-      exec_any tid s p1 r s' ->
+      exec_any restricted_step tid s p1 r s' ->
       follows_protocol_proc tid s' (p2 r)) ->
     follows_protocol_proc tid s (Bind p1 p2)
   | FollowsProtocolProcUntil :
@@ -101,7 +52,7 @@ Section Protocol.
       follows_protocol_proc tid s' (p v')) ->
     (forall s' s'' r v',
       loopInv s' tid ->
-      exec_any tid s' (p v') r s'' ->
+      exec_any restricted_step tid s' (p v') r s'' ->
       loopInv s'' tid) ->
     follows_protocol_proc tid s (Until c p v)
   | FollowsProtocolProcLog :
